\documentclass[10pt,a4paper]{article}
\usepackage[utf8x]{inputenc}
\usepackage{ucs}
\usepackage{ngerman}
\usepackage{amsmath}
\usepackage{amsfonts}
\usepackage{amssymb}
\usepackage{fancyhdr}

\author{Tilman Bender   Matrikelnummer: 108011247244\\}
\title{Einführung in Kryptographie und Datensicherheit Übung 7}

\begin{document}
\maketitle

\section*{Aufgabe 3}
\subsection*{a)}
\begin{align*}
A(x)*B(x) &= (x^{3}+x^{2}+1)*(x^{3}+x)\\
		&=x^{4}+x^{5}+\not{x^{3}}+\not{x^{3}}+x\\
		&=x^{5}+x^{4}+x
\end{align*}
\begin{align*}
(x^{5}+x^{4}+x)&:(x^{4}+x^{3}+1)=x\\
\underline{x^{5}+x^{4}+x}&\\
0
\end{align*}
\subsection*{b)}
\begin{align*}
A(x)*B(x) &= (x+1)(x^{3}+1)\\
		&=x^{4}+x+x^{3}+1\\
\end{align*}
\begin{align*}
(x^{4}+x^{3}+x+1)&:(x^{4}+x^{3}+1)=1\\
\underline{x^{4}+x^{3}+   +1}&\\
x
\end{align*}

\subsection*{c)}
\begin{align*}
A(x)*B(x) &=(x^{3}+x^{2}+x+1)(x^{3}+x^{2})\\
		&=x^{5}+x^{5}+x^{4}+x^{4}+x^{3}+x^{3}\\
		&=\not{x^{5}}+\not{x^{5}}+\not{x^{4}}+\not{x^{4}}+\not{x^{3}}+\not{x^{3}}\\
		&=0
\end{align*}
\end{document}