\documentclass[10pt,a4paper]{article}
\usepackage[utf8x]{inputenc}
\usepackage{ucs}
\usepackage{ngerman}
\usepackage{amsmath}
\usepackage{amsfonts}
\usepackage{amssymb}
\usepackage{fancyhdr}

\author{Tilman Bender   Matrikelnummer: 108011247244\\}
\title{Einführung in Kryptographie und Datensicherheit Übung 7}

\begin{document}
\maketitle

\section*{Aufgabe 2}
\subsection*{a)}
\begin{align*}
A(x)+B(x) &= (x^{3}+x^{2}+1)+(x^{3}+x+1)\\
		&=(\not{x^{3}}+x^{2}+\not{1})+(\not{x^{3}}+x+\not{1})\\
		&=x^{2}+x
\end{align*}
\subsection*{b)}
\begin{align*}
A(x)+B(x) &= (x+1)+(x^{3}+x)\\
		&= (\not{x}+1)+(x^{3}+\not{x})\\
		&=x^{3}+1
\end{align*}
\subsection*{c)}
\begin{align*}
A(x)+B(x) &=  (x^{3}+x^{2}+x+1)+(x^{3}+x)\\
		&= (\not{x^{3}}+x^{2}+\not{x}+1)+(\not{x^{3}}+\not{x})\\
		&=x^{2}+1
\end{align*}

\subsection*{d)}
Das Reduktionspolynom hat keinen Einfluss, da \dots


\end{document}